TM/LM/StepTM.v
@@ -1,2 +1,161 @@
 Require Import HeapTM.
 Require Import LookupTM JumpTargetTM.
+Require Import MatchList TokTM.
+
+
+(** ** Step semantics *)
+
+
+Section Semantics.
+
+  Implicit Types H : Heap.
+  Implicit Types T V : list HClos.
+  Implicit Types a b c : HAd.
+  Implicit Types g : HClos.
+  Implicit Types (P Q : Pro).
+
+  Definition put H e := (H++[e],|H|).
+  Definition get H a := nth_error H a.
+
+  Definition tailRecursion P a T : list HClos :=
+    match P with
+    | [] => T
+    |  _ => (P, a) :: T
+    end.
+
+
+  Definition state : Type := list HClos * list HClos * Heap.
+  
+
+  Inductive step : state -> state -> Prop :=
+  | step_pushVal P P' Q a T V H :
+      jumpTarget O [] P = Some (Q, P') ->
+      step (((lamT :: P), a) :: T, V, H) (tailRecursion P' a T, (Q, a) :: V, H)
+  | step_beta a b g P Q H H' c T V :
+      put H (Some (g, b)) = (H', c) ->
+      step (((appT :: P), a) :: T, g :: (Q, b) :: V, H) ((Q, c) :: tailRecursion P a T, V, H')
+  | step_load P a x g T V H :
+      lookup H a x = Some g ->
+      step (((varT x :: P), a) :: T, V, H) (tailRecursion P a T, g :: V, H)
+  .
+
+  Definition step_fun : state -> option state :=
+    fun '(T, V, H) =>
+      match T with
+      | ((lamT :: P), a) :: T =>
+        match jumpTarget O [] P with
+        | Some (Q, P') =>
+          Some (tailRecursion P' a T, (Q, a) :: V, H)
+        | _ => None
+        end
+      | ((appT :: P), a) :: T =>
+        match V with
+        | g :: (Q, b) :: V =>
+          let (H', c) := put H (Some (g, b)) in
+          Some ((Q, c) :: tailRecursion P a T, V, H')
+        | _ => None
+        end
+      | ((varT x :: P), a) :: T =>
+        match lookup H a x with
+        | Some g => Some (tailRecursion P a T, g :: V, H)
+        | _ => None
+        end
+      | _ => None
+      end.
+
+  Goal forall s s', step s s' -> step_fun s = Some s'.
+  Proof.
+    induction 1; cbn; TMSimp; auto.
+    unfold put in *. now inv_pair.
+  Qed.
+
+End Semantics.
+      
+
+
+
+(** ** Step Machine *)
+
+
+Section StepMachine.
+
+(** Here we compose the [Lookup] and [JumpTarget] machines, together with some matches.
+The semantics of the step machine are only defined, similarly to [Lookup] and [JumpTarget], when the simulated heap machine steps.
+
+The machine operates on lists of closures and on a heap.
+However, because [Lookup] requires an additional [sigOption sigHEnt], the alphabet also has to be extended by [sigOption sigHEnt].
+*)
+
+  Variable sigStep : finType.
+  Variable retr_closures_step : Retract (sigList sigHClos) sigStep.
+  Variable retr_heap_step : Retract sigHeap sigStep.
+  Variable retr_optHEnt_step : Retract (sigOption sigHEnt) sigStep.
+
+
+  Local Definition retr_clos_step : Retract sigHClos sigStep := ComposeRetract _ retr_closures_step.
+  Local Definition retr_pro_step : Retract sigPro sigStep := ComposeRetract _ retr_closures_step.
+  Local Definition retr_tok_step : Retract sigTok sigStep := ComposeRetract _ retr_closures_step.
+
+
+  (** Instance of the [Lookup] and [JumpTarget] machine *)
+  Local Definition Step_Lookup := Lookup retr_heap_step retr_optHEnt_step.
+  Local Definition Step_JumpTarget := ChangeAlphabet JumpTarget retr_pro_step.
+
+
+
+
+  Definition Step_lam : pTM sigStep^+ unit 11.
+  Admitted.
+
+  Definition Step_app : pTM sigStep^+ unit 11.
+  Admitted.
+
+  Definition Step_var : pTM sigStep^+ unit 11.
+  Admitted.
+
+
+  Definition Step : pTM sigStep^+ unit 11 :=
+    If (MatchList sigHClos_fin ⇑ _ @ [|Fin0; Fin3|])
+       (MatchPair sigPro_fin sigHAd_fin ⇑ retr_clos_step @ [|Fin3; Fin4|];;
+        If (MatchList sigTok_fin ⇑ retr_pro_step @ [|Fin4; Fin5|])
+           (MATCH (MatchTok ⇑ retr_tok_step @ [|Fin5|])
+                  (fun t : option ATok =>
+                     match t with
+                     | Some lamAT =>
+                       Step_lam
+                     | Some appAT =>
+                       Step_app
+                     | Some retAT =>
+                       Nop default
+                     | None (* Variable *) =>
+                       Step_var
+                     end)
+           )
+           (Nop default)
+       )
+       (Nop default)
+  .
+  
+
+
+  Definition Step_Rel : pRel sigStep^+ unit 11 :=
+    ignoreParam (
+        fun tin tout =>
+          forall (T : list HClos) (V : list HClos) (H : Heap) (T' : list HClos) (V' : list HClos) (H' : Heap),
+            step (T, V, H) (T', V', H') ->
+            tin[@Fin0] ≃ T ->
+            tin[@Fin1] ≃ V ->
+            tin[@Fin2] ≃ H ->
+            (forall i : Fin.t 8, isRight tin[@Fin.R 3 i]) ->
+            tout[@Fin0] ≃ T' /\
+            tout[@Fin1] ≃ V' /\
+            tout[@Fin2] ≃ H' /\
+            (forall i : Fin.t 8, isRight tout[@Fin.R 3 i])
+      ).
+
+
+  Lemma Step_Realise : Step ⊨ Step_Rel.
+  Admitted.
+
+
+End StepMachine.
